src/dafny/beacon/forkchoice/ForkChoiceProofs.p.dfy
@@ -39,7 +39,6 @@ module ForckChoiceProofs {
     import opened BeaconHelpers
     import opened BeaconChainTypes
     import opened ForkChoiceHelpersProofs
-    // import opened EpochProcessingProofs
 
     /**
      *  RuleI for slashing. 
@@ -53,42 +52,17 @@ module ForckChoiceProofs {
 
 
     /**
-     *  No two justified checkpoints at the same epoch.
+     *  Assume two chains from br1 and br2.
+     *  There cannot be two justified checkpoints in the two chains
+     *  at the same epoch without breaking 1/3-slashability.
+     *
+     *  @param  br1     A block root.
+     *  @param  br2     A block root.
+     *  @param  store   A store.
+     *  @param  j       An epoch.
+     *  @param  
      */
-    lemma lemma4_11(br1: Root, br2: Root, store: Store, j: nat)
-        /** The block root must be from an accepted block, i.e. in the store. */
-        requires br1 in store.blocks.Keys
-        requires br2 in store.blocks.Keys
-
-        // requires 0 <= j < 
-
-        // re
-        // requires b1 != br2 
-        /** The store is well-formed, each block with slot !=0 has a parent
-            which is itself in the store. */
-        requires forall k :: k in store.blocks.Keys && store.blocks[k].slot > 0 ==>
-            store.blocks[k].parent_root in store.blocks.Keys
-            && store.blocks[store.blocks[k].parent_root].slot < store.blocks[k].slot 
-        ensures true
-        ensures     var roots1 := chainRoots(br1, store); //  chain(br1)
-                    var roots2 := chainRoots(br2, store); //  chain(br2)
-                    var sl1 := store.blocks[roots1[0]].slot;  //  slot of br1 as a block
-                    var sl2 := store.blocks[roots2[0]].slot;  //  slot of br2 as a block
-                    //  compute the indices of EBBs in roots.
-                    var ebbsIndices1 := computeAllEBBsIndices(roots1, compute_epoch_at_slot(sl1), store);
-                    var ebbsIndices2 := computeAllEBBsIndices(roots2, compute_epoch_at_slot(sl2), store);
-                    //  given 0 <= j < compute_epoch_at_slot(sl), (roots[j],j) is the EBB at
-                    //  epoch(B) - j
-                    true
-
-    {
-        // assert();
-    }
-
-    /**
-     *  Assume two chains
-     */
-    lemma lemma4_11_a(br1: Root, br2: Root, store: Store, j: Epoch, links : seq<PendingAttestation>)
+    lemma lemma4_11_a(br1: Root, br2: Root, store: Store, j: Epoch)
          /** The block roots must be from accepted blocks, i.e. in the store. */
         requires br1 in store.blocks.Keys
         requires br2 in store.blocks.Keys
@@ -107,7 +81,7 @@ module ForckChoiceProofs {
             var k1 := computeAllEBBsIndices(chbr1, j, store);
             //  EBB(br1, j) is k1[0]
             var k2 := computeAllEBBsIndices(chbr2, j, store);
-            isJustified(0, chbr1, k1, links) && isJustified(0, chbr2, k2, links)
+            isJustified(0, chbr1, k1, store.attestations) && isJustified(0, chbr2, k2, store.attestations)
 
         ensures 
             var chbr1 := chainRoots(br1, store);
@@ -118,7 +92,7 @@ module ForckChoiceProofs {
             var k2 := computeAllEBBsIndices(chbr2, j, store);
             var tgt1 := CheckPoint(0 as Epoch, chbr1[k1[0]]);
             var tgt2 := CheckPoint(0 as Epoch, chbr2[k2[0]]);
-            |collectAttestationsForTarget(links, tgt1) * collectAttestationsForTarget(links, tgt2)|
+            |collectValidatorsIndicesAttestatingForTarget(store.attestations, tgt1) * collectValidatorsIndicesAttestatingForTarget(store.attestations, tgt2)|
             >= MAX_VALIDATORS_PER_COMMITTEE / 3 + 1
     {
         var chbr1 : seq<Root> := chainRoots(br1, store); //  chain(br1)
@@ -130,17 +104,17 @@ module ForckChoiceProofs {
         var k2 := computeAllEBBsIndices(chbr2, j, store);
         //  EBB(br2, j) is k2[0]
 
-        if (isJustified(0, chbr1, k1, links) && isJustified(0, chbr2, k2, links)) {
-            justifiedMustHaveTwoThirdIncoming(0, chbr1, k1, links);
+        if (isJustified(0, chbr1, k1, store.attestations) && isJustified(0, chbr2, k2, store.attestations)) {
+            justifiedMustHaveTwoThirdIncoming(0, chbr1, k1, store.attestations);
             var tgt1 :=  CheckPoint(0 as Epoch, chbr1[k1[0]]);
-            var attForTgt1 := collectAttestationsForTarget(links, tgt1);
+            var attForTgt1 := collectValidatorsIndicesAttestatingForTarget(store.attestations, tgt1);
             assert(|attForTgt1| >= (2 * MAX_VALIDATORS_PER_COMMITTEE) / 3 + 1);
-            justifiedMustHaveTwoThirdIncoming(0, chbr2, k2, links);
+            justifiedMustHaveTwoThirdIncoming(0, chbr2, k2, store.attestations);
             var tgt2 := CheckPoint(0 as Epoch, chbr2[k2[0]]);
-            var attForTgt2 := collectAttestationsForTarget(links, tgt2);
+            var attForTgt2 := collectValidatorsIndicesAttestatingForTarget(store.attestations, tgt2);
             assert(|attForTgt2| >= (2 * MAX_VALIDATORS_PER_COMMITTEE) / 3 + 1);
 
-            foo107(links, tgt1, tgt2);
+            supermajorityForSameEpoch(store.attestations, tgt1, tgt2);
             //  If the two blocks are the same, more than 2/3 threshold is 
             //  reached.
             if (br1 == br2) {
@@ -155,35 +129,25 @@ module ForckChoiceProofs {
     }
 
     /**
-     *  If two aggregation bits have nore than 2/3 of  MAX_VALIDATORS_PER_COMMITTEE
-     *  set to true, then the bitwise intersection of `xa` and `xb` has more than 
-     *  1/3 values et to true.
+     *  Two checkpoints with the same epoch.
+     *  Assume they both have A1 and A2 attestations more than 2/3 of total incoming attestations. 
+     *  Then the set of validators attesting for both of them has more than 1/3 total.
      *
-     *  @param  xa  A vector of bools.
-     *  @param  xb  A vector of bools.
+     *  @param  xa      A list of attestations.
+     *  @param  tgt1    A checkpoint.
+     *  @param  tgt2    A checkpoint.
      */
-    lemma foo101(xa : AggregationBits, xb: AggregationBits) 
-        // requires |xa| == |xb|
-        requires |trueBitsCount(xa)| >= (2 * MAX_VALIDATORS_PER_COMMITTEE) / 3 + 1  
-        requires |trueBitsCount(xb)| >= (2 * MAX_VALIDATORS_PER_COMMITTEE) / 3 + 1 
-        ensures |trueBitsCount(xa) * trueBitsCount(xb)| >= MAX_VALIDATORS_PER_COMMITTEE / 3 + 1
-    {
-        var k := set x: nat | 0 <= x < MAX_VALIDATORS_PER_COMMITTEE :: x;
-        successiveNatSetCardBound(k, MAX_VALIDATORS_PER_COMMITTEE);
-        assert(|k| == MAX_VALIDATORS_PER_COMMITTEE);
-        pigeonHolePrinciple(trueBitsCount(xa), trueBitsCount(xb), k);
-    }
-
-    lemma foo107(xa : seq<PendingAttestation>, tgt1: CheckPoint, tgt2: CheckPoint) 
+    lemma supermajorityForSameEpoch(xa : seq<PendingAttestation>, tgt1: CheckPoint, tgt2: CheckPoint) 
         requires tgt1.epoch == tgt2.epoch 
-        requires |collectAttestationsForTarget(xa, tgt1)| >= (2 * MAX_VALIDATORS_PER_COMMITTEE) / 3 + 1  
-        requires |collectAttestationsForTarget(xa, tgt2)| >= (2 * MAX_VALIDATORS_PER_COMMITTEE) / 3 + 1  
-        ensures |collectAttestationsForTarget(xa, tgt1) * collectAttestationsForTarget(xa, tgt2)| >= MAX_VALIDATORS_PER_COMMITTEE / 3 + 1
+        requires |collectValidatorsIndicesAttestatingForTarget(xa, tgt1)| >= (2 * MAX_VALIDATORS_PER_COMMITTEE) / 3 + 1  
+        requires |collectValidatorsIndicesAttestatingForTarget(xa, tgt2)| >= (2 * MAX_VALIDATORS_PER_COMMITTEE) / 3 + 1  
+
+        ensures |collectValidatorsIndicesAttestatingForTarget(xa, tgt1) * collectValidatorsIndicesAttestatingForTarget(xa, tgt2)| >= MAX_VALIDATORS_PER_COMMITTEE / 3 + 1
     {
         var k := set x: nat | 0 <= x < MAX_VALIDATORS_PER_COMMITTEE :: x;
         successiveNatSetCardBound(k, MAX_VALIDATORS_PER_COMMITTEE);
         assert(|k| == MAX_VALIDATORS_PER_COMMITTEE);
-        pigeonHolePrinciple(collectAttestationsForTarget(xa, tgt1), collectAttestationsForTarget(xa, tgt2), k);
+        pigeonHolePrinciple(collectValidatorsIndicesAttestatingForTarget(xa, tgt1), collectValidatorsIndicesAttestatingForTarget(xa, tgt2), k);
     }
 
 }
